# L4 Uge 8

## 1

### 1.7 Opg 1

Use a direct proof to show that the sum of two odd integers is even.

Definition

1. $n$ is even $\Leftrightarrow \exists k \in \Z : n = 2k$
2. $n$ is odd  $\Leftrightarrow \exists k \in \Z : n = 2k + 1$

Proof: (Direct proof)
$n$ is odd, $m$ is odd

$n = 2k + 1$

$m = 2l + 1$

$n + m = 2k + 1 + 2l + 1$

$n + m = 2k + 2l + 2$

$n + m = 2(k + l + 1)$

$(k + l + 1) \in \Z$

$n + m$ is even

$\square$

### 1.7 Opg 18

Prove that if m and n are integers and mn is even, then m
is even or n is even

Definition

1. $n$ is even $\Leftrightarrow \exists k \in \Z : n = 2k$
2. $n$ is odd  $\Leftrightarrow \exists k \in \Z : n = 2k + 1$

Proof: (Proof by Contradiction)

$((m = 2k + 1) \land (n = 2l + 1))\Rightarrow(\exists j\in \Z: mn=2j)$

$m = 2k + 1$

$n = 2l + 1$

$mn = (2k + 1)(2l + 1)$

$mn = 4kl + 2k + 2l + 1$

$mn = 2(2kl + k + l) + 1$

$2(2kl + k + l) + 1 = 2j \Rightarrow\Leftarrow$

$\square$

### 1.7 Opg 29

Prove that if n is a positive integer, then n is odd if and
only if 5n + 6 is odd.

### 1.7 Opg 36

Is this reasoning for finding the solutions of the equation $\sqrt{2x^2 − 1} = x$ correct?

(1) $\sqrt{2x^2 − 1} = x$ is given; $\checkmark$

(2) $2x^2 − 1 = x^2$, obtained by squaring both sides of (1); $\checkmark$

(3) $x^2 − 1 = 0$, obtained by subtracting x2 from both sides of (2); $\checkmark$

(4) $(x − 1)(x + 1) = 0$, obtained by factoring the left-hand side of $x^2 − 1$; $\checkmark$

(5) $x = 1$ or $x = −1$, which follows because $ab = 0$ implies that $a = 0$ or $b = 0$. $\checkmark$

- Yes

## 2

### 1.7 Opg 43

Prove that if n is an integer, these four statements are
equivalent:

(i) $n$ is even,

- $n$ is even $\Rightarrow \exists k \in \Z: n = 2k$

(ii) $n + 1$ is odd,

- $m$ is odd $\Rightarrow \exists k \in \Z: m = 2k +1$
- $n = 2k \Rightarrow n + 1 = 2k + 1$

(iii) $3n + 1$ is odd,

- $n = 2k \Rightarrow 3n + 1 = 3(2k) + 1$
- $\Rightarrow 3n + 1 = 6k + 1$
- $\Rightarrow 3n + 1 = 2(3k) + 1$
- $3k \in \Z$

(iv) 3n is even.

- $n = 2k \Rightarrow 3n = 3 (2k)$
- $\Rightarrow 3n = 6k$
- $\Rightarrow 3n = 2(3k)$
- $3k \in \Z$
